\documentclass{article}
\pagestyle{empty}
\usepackage{prooftree}
\usepackage{xspace,amssymb,amsfonts,amsmath,color}
\usepackage{mathptmx}
\begin{document}
\begin{displaymath}
\prooftree
\prooftree
\prooftree
\prooftree
\prooftree
\justifies
p \vdash ((q \to r) \lor s), p \ \ \ 
\using
(AX)
\endprooftree
\prooftree
\prooftree
\justifies
s \vdash p, (q \to r), s \ \ \ 
\using
(AX)
\endprooftree
\justifies
s \vdash p, ((q \to r) \lor s) \ \ \ 
\using
(\lor R)
\endprooftree
\justifies
(p \lor s) \vdash ((q \to r) \lor s), p \ \ \ 
\using
(\lor L)
\endprooftree
\justifies
 \vdash p, ((p \lor s) \to ((q \to r) \lor s)) \ \ \ 
\using
(\to R)
\endprooftree
\prooftree
\prooftree
\prooftree
\prooftree
\prooftree
\prooftree
\justifies
q, p \vdash r, q, s \ \ \ 
\using
(AX)
\endprooftree
\justifies
p \vdash q, s, (q \to r) \ \ \ 
\using
(\to R)
\endprooftree
\justifies
p \vdash q, ((q \to r) \lor s) \ \ \ 
\using
(\lor R)
\endprooftree
\prooftree
\prooftree
\justifies
s \vdash q, (q \to r), s \ \ \ 
\using
(AX)
\endprooftree
\justifies
s \vdash q, ((q \to r) \lor s) \ \ \ 
\using
(\lor R)
\endprooftree
\justifies
(p \lor s) \vdash ((q \to r) \lor s), q \ \ \ 
\using
(\lor L)
\endprooftree
\justifies
 \vdash q, ((p \lor s) \to ((q \to r) \lor s)) \ \ \ 
\using
(\to R)
\endprooftree
\prooftree
\prooftree
\prooftree
\prooftree
\prooftree
\justifies
q, p, r \vdash r, s \ \ \ 
\using
(AX)
\endprooftree
\justifies
p, r \vdash s, (q \to r) \ \ \ 
\using
(\to R)
\endprooftree
\justifies
p, r \vdash ((q \to r) \lor s) \ \ \ 
\using
(\lor R)
\endprooftree
\prooftree
\prooftree
\justifies
r, s \vdash (q \to r), s \ \ \ 
\using
(AX)
\endprooftree
\justifies
r, s \vdash ((q \to r) \lor s) \ \ \ 
\using
(\lor R)
\endprooftree
\justifies
r, (p \lor s) \vdash ((q \to r) \lor s) \ \ \ 
\using
(\lor L)
\endprooftree
\justifies
r \vdash ((p \lor s) \to ((q \to r) \lor s)) \ \ \ 
\using
(\to R)
\endprooftree
\justifies
(q \to r) \vdash ((p \lor s) \to ((q \to r) \lor s)) \ \ \ 
\using
(\to L)
\endprooftree
\justifies
(p \to (q \to r)) \vdash ((p \lor s) \to ((q \to r) \lor s)) \ \ \ 
\using
(\to L)
\endprooftree
\justifies
 \vdash ((p \to (q \to r)) \to ((p \lor s) \to ((q \to r) \lor s))) \ \ \ 
\using
(\to R)
\endprooftree
\end{displaymath}
\end{document}